Adapt the compiler to the typed code generator

CertSkel/CUDALib.v
@@ -13,6 +13,7 @@ Definition locs ty := typ2Coq loc ty.
 Definition ctys ty := typ2Coq (option CTyp) ty.
 Definition exps ty := typ2Coq exp ty.
 Definition lexps ty := typ2Coq loc_exp ty.
+Definition vartys ty := typ2Coq (var * CTyp) ty.
 
 Fixpoint nleaf ty :=
   match ty with
@@ -50,13 +51,13 @@ Fixpoint writes {ty : Skel.Typ} :=
     writes (fst les) (fst es) ;; writes (snd les) (snd es)
   end.
 
-Fixpoint nat_to_string (n : nat) : string :=
+Fixpoint nat2str (n : nat) : string :=
   match n with
   | O => "O"
-  | S n => "S" ++ nat_to_string n
+  | S n => "S" ++ nat2str n
   end%string.
 
-Lemma nat_to_string_inj n m : nat_to_string n = nat_to_string m -> n = m.
+Lemma nat_to_string_inj n m : nat2str n = nat2str m -> n = m.
 Proof.
   revert m; induction n; simpl in *; intros [|m]; simpl; try congruence.
   inversion 1. eauto.
@@ -68,3 +69,45 @@ Proof.
   revert s1'; induction s1; intros [|? s1']; simpl in *; try congruence; intros.
   inverts H; inverts H0; subst; eauto.
 Qed.
+
+Fixpoint locs_offset {ty} :=
+  match ty return lexps ty -> exp -> lexps ty with
+  | Skel.TBool | Skel.TZ => loc_offset
+  | Skel.TTup t1 t2 => fun l off => (locs_offset (fst l) off, locs_offset (snd l) off)
+  end.
+
+Infix "+os" := (locs_offset) (at level 50, left associativity).
+
+Fixpoint maptys {ty T1 T2} (f : T1 -> T2) :=
+  match ty return typ2Coq T1 ty -> typ2Coq T2 ty with
+  | Skel.TBool | Skel.TZ => fun x => f x
+  | Skel.TTup t1 t2 => fun xs =>
+    (maptys f (fst xs), maptys f (snd xs))
+  end.
+
+Definition v2e {ty} := @maptys ty _ _ Evar.
+Definition e2sh {ty} := @maptys ty _ _ Sh.
+Definition e2gl {ty} := @maptys ty _ _ Gl.
+Definition v2sh {ty} (xs : vars ty) := (e2sh (v2e xs)).
+Definition v2gl {ty} (xs : vars ty) := (e2sh (v2e xs)).
+
+Fixpoint ty2ctys ty :=
+  match ty return ctys ty with
+  | Skel.TBool => Some Bool
+  | Skel.TZ => Some Int
+  | Skel.TTup t1 t2 => (ty2ctys t1, ty2ctys t2)
+  end.
+
+Definition names_of_array grp d := ls_init 0 d (fun i => "arr" ++ grp ++ nat2str i)%string.
+Definition name_of_len grp := ("sh" ++ grp)%string.
+Definition names_of_arg grp d := (name_of_len grp, names_of_array grp d).
+
+Definition grpOfInt n := ("In" ++ nat2str n)%string.
+
+Close Scope string.
+
+Fixpoint flatTup {ty : Skel.Typ} {T : Type} :=
+  match ty return typ2Coq T ty -> list T with
+  | Skel.TBool | Skel.TZ => fun x => x :: nil
+  | Skel.TTup _ _ => fun xs => flatTup (fst xs) ++ flatTup (snd xs)
+  end.
